LogicalRefinement/Typed/Regular.lean
@@ -84,13 +84,20 @@ theorem HasType.regular (p: Γ ⊢ a: A): A.regular Γ := by {
       exact Hψ.upgrade
       assumption
 
-  case inst => sorry
+  case inst Hf Hl Hr If Il Ir => 
+    constructor
+    apply HasType.downgrade
+    apply HasType.subst0_sort
+    cases Hf with
+    | forall_ HA Hφ => exact Hφ.upgrade
+    assumption
 
   case let_wit => sorry
 
   case refl Ha IA =>  
     cases IA;
     constructor
+    apply HasType.downgrade
     constructor
     assumption
     apply HasType.upgrade
